Prove more lemmas in hoas.v

sandbox/hoas.v
@@ -6,6 +6,8 @@ Reserved Notation "x * y" (at level 40, left associativity).
 Reserved Notation "x 'o' y" (at level 30, right associativity).
 Reserved Notation "x || y" (at level 50, left associativity).
 Reserved Notation "x (+) y" (at level 45, no associativity).
+Reserved Notation "x @ f" (at level 55, right associativity).
+Reserved Notation "cf *@ x" (at level 55, right associativity).
 Reserved Notation "x [= y" (at level 60, no associativity).
 Reserved Notation "x [=] y" (at level 60, no associativity).
 Reserved Notation "x [!= y" (at level 60, no associativity).
@@ -48,15 +50,7 @@ Notation "x 'o' y" := (code_b * x * y)%code : code_scope.
 Notation "x || y" := (code_j * x * y)%code : code_scope.
 
 Inductive beta {Var : Set} : Code Var -> Code Var -> Prop :=
-  | beta_refl x : beta x x
-  | beta_trans x y z : beta x y -> beta y z -> beta x z
-  | beta_ap_left x x' y : beta x x' -> beta (x * y) (x' * y)
-  | beta_ap_right x y y' : beta y y' -> beta (x * y) (x * y')
-  | beta_top x : beta TOP x
-  | beta_bot x : beta x BOT
   | beta_j x y z : beta ((x || y) * z) (x * z || y * z)
-  | beta_j_left x y : beta (x || y) x
-  | beta_j_right x y : beta (x || y) y
   | beta_i x : beta (I * x) x
   | beta_k x y : beta (K * x * y) x
   | beta_b x y z : beta (B * x * y * z) (x * (y * z))
@@ -64,9 +58,27 @@ Inductive beta {Var : Set} : Code Var -> Code Var -> Prop :=
   | beta_s x y z : beta (S * x * y * z) (x * z * (y * z))
   | beta_y x : beta (Y * x) (x * (Y * x))
   | beta_v x : beta (V * x) (I || x o (V * x)).
-Hint Constructors beta.
 
-Fixpoint try_beta_step {Var : Set} (u : Code Var) : option (Code Var) :=
+Inductive pi {Var : Set} : Code Var -> Code Var -> Prop :=
+  | pi_top x : pi TOP x
+  | pi_bot x : pi x BOT
+  | pi_j_left x y : pi (x || y) x
+  | pi_j_right x y : pi (x || y) y.
+
+Inductive red {Var : Set} : Code Var -> Code Var -> Prop :=
+  | red_refl x : red x x
+  | red_trans x y z : red x y -> red y z -> red x z
+  | red_ap_left x x' y : red x x' -> red (x * y) (x' * y)
+  | red_ap_right x y y' : red y y' -> red (x * y) (x * y')
+  | red_beta x y : beta x y -> red x y
+  | red_beta' x y : beta y x -> red x y
+  | red_pi x y : pi x y -> red x y.
+
+Hint Constructors beta.
+Hint Constructors pi.
+Hint Constructors red.
+
+Fixpoint try_red_step {Var : Set} (u : Code Var) : option (Code Var) :=
   match u with
   | I * x => Some x
   | K * x * y => Some x
@@ -77,10 +89,10 @@ Fixpoint try_beta_step {Var : Set} (u : Code Var) : option (Code Var) :=
   | Y * x => Some (x * (Y * x))
   | V * x => Some (I || x o (V * x))
   | x * y =>
-      match try_beta_step x with
+      match try_red_step x with
       | Some x' => Some (x' * y)
       | None =>
-          match try_beta_step y with
+          match try_red_step y with
           | Some y' => Some (x * y')
           | None => None
           end
@@ -88,41 +100,43 @@ Fixpoint try_beta_step {Var : Set} (u : Code Var) : option (Code Var) :=
   | _ => None
   end.
 
-Section try_beta_step.
+Section try_red_step.
   Variable Var : Set.
   Variable x : Code Var.
   Eval compute in
-    (try_beta_step ((x || (C * I * TOP) o (V * (C * I * TOP)) * x))).
-End try_beta_step.
+    (try_red_step ((x || (C * I * TOP) o (V * (C * I * TOP)) * x))).
+End try_red_step.
 
-Ltac beta_to x := apply beta_trans with x; auto.
+Ltac red_to x := apply red_trans with x; auto.
 
-Ltac beta_step_ try_beta_step :=
+Ltac red_step_ try_red_step :=
   match goal with
-  | [|- @beta ?v ?x ?y] =>
-      match eval compute in (try_beta_step v x) with
-      | Some ?z => beta_to z
+  | [|- @red ?v ?x ?y] =>
+      match eval compute in (try_red_step v x) with
+      | Some ?z => red_to z
       | _ => fail
       end
   | _ => fail
   end.
 
-Ltac beta_step := beta_step_ @try_beta_step.
+Ltac red_step := red_step_ @try_red_step.
 
 Definition code_div {Var : Set} : Code Var := V * (C * I * TOP).
-Lemma beta_div {Var : Set} (x : Code Var) :
-  beta (code_div * x) (x || code_div * x * TOP).
+Lemma red_div {Var : Set} (x : Code Var) :
+  red (code_div * x) (x || code_div * x * TOP).
 Proof.
   unfold code_div.
-  beta_step.
-  beta_step.
-  beta_step.
-  apply beta_ap_right. (* FIXME allow variables in beta_step *)
-  beta_step.
-  beta_step.
+  red_step.
+  red_step.
+  red_step.
+  apply red_ap_right. (* FIXME allow variables in red_step *)
+  red_step.
+  red_step.
 Qed.
 
-Definition conv {Var : Set} (x : Code Var) := beta (code_div * x) TOP.
+Definition conv {Var : Set} (x : Code Var) := red (code_div * x) TOP.
+
+Ltac conv_to x := unfold conv; red_to x; fold conv.
 
 (** ** Substitution and abstraction *)
 
@@ -144,7 +158,9 @@ Fixpoint code_sub {Var Var' : Set}
   end.
 Hint Resolve code_sub.
 
-Lemma var_monad_unit (Var : Set) (x : Code Var) : code_sub code_var x = x.
+Notation "x @ f" := (code_sub f x)%code : code_scope.
+
+Lemma var_monad_unit (Var : Set) (x : Code Var) : x @ code_var = x.
 Proof.
   induction x; auto.
   unfold code_sub; fold (@code_sub Var Var).
@@ -152,9 +168,15 @@ Proof.
 Qed.
 
 Lemma var_monad_unit_left (Var Var' : Set) (f : Var -> Code Var') x :
-  code_sub f (code_var x) = f x.
+  (code_var x) @ f = f x.
 Proof.
   compute; auto.
+Qed.
+
+Lemma code_sub_ap (Var Var' : Set)
+  (x y : Code Var) (f : Var -> Code Var') : (x * y @ f) = (x @ f) * (y @ f).
+Proof.
+  simpl; auto.
 Qed.
 
 Lemma var_monad_assoc
@@ -162,136 +184,158 @@ Lemma var_monad_assoc
   (f : Var -> Code Var')
   (g : Var' -> Code Var'')
   (x : Code Var) :
-  code_sub g (code_sub f x) = code_sub (fun v => code_sub g (f v)) x.
+  (x @ f) @ g = x @ (fun v => (f v) @ g).
 Proof.
-  (* TODO *)
-Admitted.
+  induction x; auto.
+  repeat rewrite code_sub_ap.
+  rewrite IHx1; rewrite IHx2; auto.
+Qed.
 
-Lemma beta_sub_left {Var Var' : Set}
-  {f g : Var -> Code Var'} (fg : forall v, beta (f v) (g v))
-  (x : Code Var) : beta (code_sub f x) (code_sub g x).
+Lemma code_sub_ext {Var Var' : Set}
+  (f g : Var -> Code Var') (fg : forall v, f v = g v) x :
+  x @ f = x @ g.
+Proof.
+  induction x; simpl; auto.
+  rewrite IHx1; rewrite IHx2; auto.
+Qed.
+
+Lemma red_sub_left {Var Var' : Set}
+  {f g : Var -> Code Var'} (fg : forall v, red (f v) (g v))
+  (x : Code Var) : red (x @ f) (x @ g).
 Proof.
   induction x; auto.
     compute; auto.
   unfold code_sub; fold (@code_sub Var Var').
-  beta_to (code_sub f x1 * code_sub g x2).
+  red_to ((x1 @ f) * (x2 @ g)).
 Defined.
-Hint Resolve beta_sub_left.
+Hint Resolve red_sub_left.
 
 Lemma beta_sub_right {Var Var' : Set}
-  (f : Var -> Code Var') (x y : Code Var) (xy : beta x y) :
-  beta (code_sub f x) (code_sub f y).
+  (f : Var -> Code Var') (x y : Code Var)
+  (xy : beta x y) : beta (x @ f) (y @ f).
 Proof.
-  induction x; inversion xy; auto.
-  (* TODO *)
-Admitted.
+  induction xy; repeat rewrite code_sub_ap; simpl; auto.
+Qed.
 Hint Resolve beta_sub_right.
 
-Lemma beta_sub {Var Var' : Set}
-  {f g : Var -> Code Var'} (fg : forall v, beta (f v) (g v))
-  {x y : Code Var} (xy : beta x y) :
-  beta (code_sub f x) (code_sub g y).
+Lemma pi_sub_right {Var Var' : Set}
+  (f : Var -> Code Var') (x y : Code Var)
+  (xy : pi x y) : pi (x @ f) (y @ f).
 Proof.
-  beta_to (code_sub g x).
+  induction xy; repeat rewrite code_sub_ap; simpl; auto.
+Qed.
+Hint Resolve pi_sub_right.
+
+Lemma red_sub_right {Var Var' : Set}
+  (f : Var -> Code Var') (x y : Code Var)
+  (xy : red x y) : red (x @ f) (y @ f).
+Proof.
+  induction xy; repeat rewrite code_sub_ap; simpl; auto.
+  apply red_trans with (y @ f); auto.
+Qed.
+Hint Resolve red_sub_right.
+
+Lemma red_sub {Var Var' : Set}
+  {f g : Var -> Code Var'} (fg : forall v, red (f v) (g v))
+  {x y : Code Var} (xy : red x y) :
+  red (code_sub f x) (code_sub g y).
+Proof.
+  red_to (code_sub g x).
 Defined.
-Hint Resolve beta_sub.
+Hint Resolve red_sub.
 
 (** Contexts, convergence, and information ordering *)
 
-(** Contexts represent linear functions of code *)
-Inductive Context (Var Var' : Set) : Set :=
-  Context_intro : (Var -> Code Var') -> Code (option Var') -> Context Var Var'.
-Definition context_intro {Var Var' : Set} := Context_intro Var Var'.
+Definition code_le {Var : Set} (x y : Code Var) :=
+  forall {Var' : Set} (c : Code Var') (f : Var -> Code Var'),
+  conv (c * (x @ f)) -> conv (c * (y @ f)).
 
-Fixpoint context_eval {Var Var' : Set}
-  (c : Context Var Var') (x : Code Var) : Code Var' :=
-  let (c1, c2) := c in
-  let x' := code_sub c1 x in
-  let f v := match v with None => x' | Some v' => code_var v' end in
-  code_sub f c2.
+Notation "x [= y" := (code_le x y)%code : code_scope.
 
-Notation "c @ x" := (context_eval c x)
-  (at level 60, no associativity) : code_scope.
-Notation "( c1 , c2 ) @ x" := (context_intro c1 c2 @ x)
-  (at level 60, no associativity) : code_scope.
-
-Lemma context_beta_right {Var Var' : Set}
-  (c : Context Var Var') (x y : Code Var) (xy : beta x y) :
-  beta (c @ x) (c @ y).
+Lemma code_le_refl {Var : Set} (x : Code Var) : x [= x.
 Proof.
-  (* TODO *)
-Admitted.
-
-Definition conv_in {Var Var' : Set}
-  (c : Context Var Var') (x : Code Var) : Prop :=
-  conv (c @ x).
-
-Definition code_le {Var : Set} (x y : Code Var) : Prop :=
-  forall (Var' : Set) (c : Context Var Var'), conv_in c x -> conv_in c y.
-
-Definition context_div {Var Var' : Set}
-  (c1 : Var -> Code Var') (c2 : Code (option Var'))
-  (x : Code Var) :
-  code_div * ((c1, c2) @ x) = (fun v => code_div * c1 v, c2) @ x.
-Proof.
-  unfold context_eval at 2; simpl.
-Admitted.
-
-Lemma code_le_x_top' {Var : Set} (c x : Code Var) :
-  beta (c * x) TOP -> beta (c * TOP) TOP.
-Proof.
-  apply beta_trans; auto.
+  unfold code_le; auto.
 Qed.
+Hint Resolve code_le_refl.
 
-Lemma code_le_x_top {Var : Set} (x : Code Var) : code_le x code_top.
+Lemma code_le_trans {Var : Set} (x y z : Code Var) :
+  x [= y -> y [= z -> x [= z .
 Proof.
-  unfold code_le; unfold conv_in; unfold conv; intros Var' c.
-  destruct c as [c1 c2].
-  repeat rewrite context_div.
-  intros Hbeta.
-  beta_to ((fun v : Var => code_div * c1 v, c2) @ x).
-  apply context_beta_right; auto.
-Defined.
-
-Lemma code_le_bot_x' {Var : Set} (c x : Code Var) :
-  beta (c * BOT) TOP -> beta (c * x) TOP.
-Proof.
-  apply beta_trans; auto.
+  unfold code_le; auto.
 Qed.
+Hint Resolve code_le_trans.
 
-Lemma code_le_bot_x {Var : Set} (x : Code Var) : code_le code_bot x.
+Lemma code_le_ap_right {Var : Set} {x y y' : Code Var} :
+  y [= y' -> x * y [= x * y'.
 Proof.
-  unfold code_le; unfold conv_in; unfold conv; intros Var' c.
-  destruct c as [c1 c2].
-  repeat rewrite context_div.
-  intros Hbeta.
-  beta_to ((fun v : Var => code_div * c1 v, c2) @ BOT).
-  apply context_beta_right; auto.
-Defined.
-
-Lemma code_le_k_j {Var : Set} : @code_le Var code_k code_j.
-Proof.
-  unfold code_le; intros Var' c Hconv.
-  induction c; simpl; auto.
-  induction Hconv.
-Admitted.
+  unfold code_le; unfold conv; intros H Var' c f.
+  repeat rewrite code_sub_ap.
+  intros Hconv.
+  red_to (code_div * ((c o (x @ f)) * (y' @ f))).
+  apply H.
+  red_to (code_div * (c * ((x @ f) * (y @ f)))).
+Qed.
+Hint Resolve code_le_ap_right.
 
 Lemma code_le_ap_left {Var : Set} {x x' y : Code Var} :
-  code_le x x' -> code_le (x * y) (x' * y).
-Admitted.
-
-Lemma code_le_ap_right {Var : Set} {x y y': Code Var} :
-  code_le y y' -> code_le (x * y) (x * y').
-Admitted.
+  x [= x' -> x * y [= x' * y.
+Proof.
+  unfold code_le; unfold conv; intros H Var' c f.
+  repeat rewrite code_sub_ap.
+  intros Hconv.
+  red_to (code_div * (c * (I * (x' @ f) * (y @ f)))).
+  red_to (code_div * (c * (C * I * (y @ f) * (x' @ f)))).
+  red_to (code_div * (c o (C * I * (y @ f)) * (x' @ f))).
+  apply H.
+  red_to (code_div * (c * (C * I * (y @ f) * (x @ f)))).
+  red_to (code_div * (c * (I * (x @ f) * (y @ f)))).
+  red_to (code_div * (c * ((x @ f) * (y @ f)))).
+Qed.
+Hint Resolve code_le_ap_left.
 
 Lemma code_le_ap {Var : Set} {x x' y y': Code Var} :
   code_le x x' -> code_le y y' -> code_le (x * y) (x' * y').
-Admitted.
+Proof.
+  intros Hx Hy.
+  apply code_le_trans with (x * y'); auto.
+Qed.
+Hint Resolve code_le_ap.
 
-Lemma code_le_subs {Var : Set} (d : Var -> bool) (x y y' : Code Var) :
-  code_le y y' -> 
-  code_le (code_sub (fun v => if d v then y else code_var v) x)
-          (code_sub (fun v => if d v then y' else code_var v) x).
+Lemma code_le_top {Var : Set} (x : Code Var) : x [= TOP.
+Proof.
+  unfold code_le; intros Var' c f Hred.
+  red_to (code_div o c * TOP).
+  red_to (code_div o c * (x @ f)).
+  red_to (code_div * (c * (x @ f))).
+Defined.
+Hint Resolve code_le_top.
+
+Lemma code_le_bot {Var : Set} (x : Code Var) : BOT [= x.
+Proof.
+  unfold code_le; intros Var' c f Hred.
+  red_to (code_div o c * (x @ f)).
+  red_to (code_div o c * BOT).
+  red_to (code_div * (c * BOT)).
+Defined.
+Hint Resolve code_le_bot.
+
+Lemma code_le_j_left {Var : Set} (x y : Code Var) : x [= x || y.
+Proof.
+  unfold code_le; intros Var' c f Hred.
+  red_to (code_div * (c * (x @ f))).
+Qed.
+
+Lemma code_le_j_right {Var : Set} (x y : Code Var) : y [= x || y.
+Proof.
+  unfold code_le; intros Var' c f Hred.
+  red_to (code_div * (c * (y @ f))).
+Qed.
+
+Lemma code_le_j {Var : Set} (x y z : Code Var) :
+  x [= z -> y [= z -> x || y [= z.
+Proof.
+  unfold code_le; intros Hx Hy Var' c f.
+  (* TODO *)
 Admitted.
 
 (** ** Curry's abstraction algorithm *)
@@ -317,16 +361,16 @@ Fixpoint code_abs {Var Var' : Set} (b : Var -> option Var') (x : Code Var) :
   | V => K * V
   end.
 
-Lemma abs_sub_beta {Var Var' : Set}
+Lemma abs_sub_red {Var Var' : Set}
   (b : Var -> option Var') (x : Code Var) (y : Code Var') :
-  beta (code_abs b x * y)
+  red (code_abs b x * y)
        (code_sub (fun v => match b v with None => y
                                         | Some v' => code_var v' end) x).
 Proof.
   induction x; simpl; auto.
     case (b v); [intro v'; auto | auto].
-  beta_to (code_abs b x1 * y * (code_abs b x2 * y)).
-  beta_to
+  red_to (code_abs b x1 * y * (code_abs b x2 * y)).
+  red_to
     (code_abs b x1 * y
     * (code_sub (fun v => match b v with None => y
                                        | Some v' => code_var v' end) x2)).
@@ -360,9 +404,9 @@ Fixpoint code_abs' {Var Var' : Set} (b : Var -> option Var') (x : Code Var) :
   | V => K * V
   end.
 
-Lemma abs_sub_beta' {Var Var' : Set}
+Lemma abs_sub_red' {Var Var' : Set}
   (b : Var -> option Var') (x : Code Var) (y : Code Var') :
-  beta (code_abs' b x * y)
+  red (code_abs' b x * y)
        (code_sub (fun v => match b v with None => y
                                         | Some v' => code_var v' end) x).
 Proof.
